finished defining SpecM as a general interface

theories/Ref/SpecM.v
@@ -13,7 +13,6 @@ From EnTree Require Import
      Eq.Eqit
      Ref.Padded
      Ref.EnTreeSpecDefinition
-     Ref.MRecSpec
      Ref.FixTree
 .
 From Coq Require Import
@@ -35,7 +34,6 @@ Import Monads.
 Import ProperNotations.
 
 
-
 (**
  ** EncodingType and ReSum instances for defining SpecM
  **)
@@ -47,7 +45,7 @@ Inductive ErrorE : Set :=
 Global Instance EncodingType_ErrorE : EncodingType ErrorE := fun _ => Empty_set.
 
 (* The event type for SpecM computations, given an underlying event type *)
-Definition SpecE (E : EvType@{entree_u}) : Type@{entree_u} :=
+Definition SpecE (E : EvType) : Type@{entree_u} :=
   SpecEvent (ErrorE + E).
 
 (* The return type for a SpecEE effect in a SpecM computation *)
@@ -74,168 +72,34 @@ Global Instance ReSumRet_SpecE_Error (E : EvType) : ReSumRet ErrorE (SpecE E) :=
  ** The SpecM monad
  **)
 
-(* The SpecM monad is an entree spec over FunStackE events *)
-Definition SpecM (E:EvType) stack A : Type :=
-  fixtree (SpecEv E) stack A.
+Section SpecM.
 
-#[global] Instance Monad_SpecM {E stk} : Monad (SpecM E stk) := Monad_fixtree.
+Context {Tp} `{IsTpDesc Tp} {E : EvType}.
+
+(* The SpecM monad is an entree spec over SpecE events *)
+Definition SpecM A : Type := fixtree Tp (SpecEv E) A.
+
+#[global] Instance Monad_SpecM : Monad SpecM := Monad_fixtree _ _.
 
 (* The monadic operations on SpecM *)
-Definition RetS {E} {stk A} (a : A) : SpecM E stk A := ret a.
-Definition BindS {E} {stk A B} (m : SpecM E stk A) (k : A -> SpecM E stk B) :=
-  bind m k.
+Definition RetS {A} (a : A) : SpecM A := ret a.
+Definition BindS {A B} (m : SpecM A) (k : A -> SpecM B) := bind m k.
 
-Definition ForallS {E} {stk} (A : Type) `{QuantType A} : SpecM E stk A :=
+Definition ForallS (A : Type) `{QuantType A} : SpecM A :=
   Fx_Vis (Spec_forall quantEnc : SpecEv E) (fun x => Fx_Ret (quantEnum x)).
-Definition ExistsS {E} {stk} (A : Type) `{QuantType A} : SpecM E stk A :=
+Definition ExistsS (A : Type) `{QuantType A} : SpecM A :=
   Fx_Vis (Spec_exists quantEnc : SpecEv E) (fun x => Fx_Ret (quantEnum x)).
 
-Definition AssumeS {E} {stk} (P : Prop) : SpecM E stk unit :=
+Definition AssumeS (P : Prop) : SpecM unit :=
   BindS (ForallS P) (fun _ => ret tt).
-Definition AssertS {E} {stk} (P : Prop) : SpecM E stk unit :=
+Definition AssertS (P : Prop) : SpecM unit :=
   BindS (ExistsS P) (fun _ => ret tt).
 
-Definition TriggerS {E:EvType} {stk} (e : E) : SpecM E stk (encodes e) :=
+Definition TriggerS (e : E) : SpecM (encodes e) :=
   Fx_Vis (resum e : SpecEv E) (fun x => Fx_Ret x).
 
-Definition ErrorS {E} {stk} A (str : string) : SpecM E stk A :=
+Definition ErrorS A (str : string) : SpecM A :=
   Fx_Vis ((Spec_vis (inl (mkErrorE str))) : SpecEv E)
     (fun (x:Empty_set) => match x with end).
 
-
-(**
- ** Making and calling tpElems
- **)
-
-(* Re-exporting tpElem from the SpecM module *)
-Definition tpElem := tpElem.
-
-(* A tpElem specifically of SpecM type *)
-Definition specElem E stk R := tpElem E stk (Tp_M R).
-
-(* A tpElem specifically of pi type *)
-Definition piElem E stk A B := tpElem E stk (Tp_Pi A B).
-
-(* A tpElem specifically of arrow type *)
-Definition arrowElem E stk A B := tpElem E stk (Tp_Arr A B).
-
-
-(* An element of a type description that uses SpecM for the monadic type *)
-Fixpoint SpecElem E stk T : Type@{entree_u} :=
-  match T with
-  | Tp_M R => SpecM E stk (tpElem (SpecEv E) stk R)
-  | Tp_Pi A B => forall a, SpecElem E stk (B a)
-  | Tp_Arr A B => tpElem (SpecEv E) stk A -> SpecElem E stk B
-  | Tp_SType A => tpElem (SpecEv E) stk (Tp_SType A)
-  | Tp_Pair A B => tpElem (SpecEv E) stk (Tp_Pair A B)
-  | Tp_Sum A B => tpElem (SpecEv E) stk (Tp_Sum A B)
-  | Tp_Sigma A B => tpElem (SpecEv E) stk (Tp_Sigma A B)
-  end.
-
-Definition PolySpecElem E stk T : Type@{entree_u} :=
-  forall stk' (incl : stackIncl stk stk'), SpecElem E stk' T.
-
-Definition liftPolySpecElem {E stk stk' T} (incl : stackIncl stk stk')
-  (elem : PolySpecElem E stk T) : PolySpecElem E stk' T :=
-  fun stk'' incl' => elem stk'' (compListIncl incl incl').
-
-Definition lift0PolySpecElem {E stk U T} (elem : PolySpecElem E stk T)
-  : PolySpecElem E (U :: stk) T :=
-  liftPolySpecElem (stepListIncl (incl1Base U stk)) elem.
-
-Definition applyPolySpecElem {E stk T U}
-  (f : PolySpecElem E stk (Tp_Arr T U)) (arg : tpElem (SpecEv E) stk T)
-  : PolySpecElem E stk U :=
-  fun stk' incl => f stk' incl (liftTpElem incl arg).
-
-Fixpoint SpecElemToMonoInterp {E stk} T : SpecElem E stk T -> MonoInterp (SpecEv E) stk T :=
-  match T return SpecElem E stk T -> MonoInterp (SpecEv E) stk T with
-  | Tp_M R => fun elem args => elem
-  | Tp_Pi A B =>
-      fun elem args =>
-        SpecElemToMonoInterp (B (projT1 args)) (elem (projT1 args)) (projT2 args)
-  | Tp_Arr A B =>
-      fun elem args =>
-        SpecElemToMonoInterp B (elem (fst args)) (snd args)
-  | Tp_SType A => fun elem args => match args with end
-  | Tp_Pair A B => fun elem args => match args with end
-  | Tp_Sum A B => fun elem args => match args with end
-  | Tp_Sigma A B => fun elem args => match args with end
-  end.
-
-Definition SpecElemToInterp {E stk T} (elem: PolySpecElem E stk T)
-  : FixTree.FxInterp (SpecEv E) stk T :=
-  fun stk' incl => @SpecElemToMonoInterp E stk' T (elem stk' incl).
-
-Fixpoint InterpToSpecElem {E stk} T
- : isFunTp T -> FxInterp (SpecEv E) stk T -> SpecElem E stk T :=
-  match T return isFunTp T -> FxInterp (SpecEv E) stk T -> SpecElem E stk T with
-  | Tp_M R => fun _ m => m stk (reflListIncl _) tt
-  | Tp_Pi A B => fun isfun f a =>
-                   InterpToSpecElem (B a) (isfun a)
-                     (fun stk' incl args => f stk' incl (existT _ a args))
-  | Tp_Arr A B =>
-      fun isfun f arg =>
-        InterpToSpecElem B isfun (fun stk' incl args =>
-                                    f stk' incl (liftTpElem incl arg, args))
-  | Tp_SType _ => fun isfun => match isfun with end
-  | Tp_Pair _ _ => fun isfun => match isfun with end
-  | Tp_Sum _ _ => fun isfun => match isfun with end
-  | Tp_Sigma _ _ => fun isfun => match isfun with end
-  end.
-
-Definition callStkFun {E stk T} (stkf : StkFun stk T) : SpecElem E stk T :=
-  match stkf with
-  | MkStkFun _ _ n isn isfun =>
-      InterpToSpecElem T isfun
-        (fun stk' incl args =>
-           Fx_Call (MkStackCall _ _ T
-                      (applyListIncl incl n) (applyListInclNth incl isn) args)
-             (fun x => Fx_Ret x))
-  end.
-
-Fixpoint CallS {E stk T} : tpElem (SpecEv E) stk T -> SpecElem E stk T :=
-  match T return tpElem (SpecEv E) stk T -> SpecElem E stk T with
-  | Tp_M R =>
-      fun elem => match elem with
-                  | inl stkf => callStkFun stkf
-                  | inr m => embedEntree m
-                  end
-  | Tp_Pi A B =>
-      fun elem => match elem with
-                  | inl stkf => callStkFun stkf
-                  | inr f => fun a => CallS (f a)
-                  end
-  | Tp_Arr A B =>
-      fun elem => match elem with
-                  | inl stkf => callStkFun stkf
-                  | inr f => fun arg => CallS (f stk (reflListIncl _) arg)
-                  end
-  | Tp_SType _ => fun elem => elem
-  | Tp_Pair _ _ => fun elem => elem
-  | Tp_Sum _ _ => fun elem => elem
-  | Tp_Sigma _ _ => fun elem => elem
-  end.
-
-
-Definition fixS {E stk T} (isfun : isFunTp T) (body : PolySpecElem E stk (Tp_Arr T T))
-  : SpecElem E stk T :=
-  InterpToSpecElem (stk:=stk) T isfun
-    (fun stk' incl args =>
-       Fx_Fix (SpecElemToInterp (liftPolySpecElem (consListIncl _ incl)
-                                   (applyPolySpecElem
-                                      (lift0PolySpecElem body)
-                                      (tpElem0 isfun))))
-         args (fun x => Fx_Ret x)).
-
-
-FIXME: how to define mkTpElem?
-
-Fixpoint mkTpElem {E stk T} : SpecElem E nil T -> tpElem (SpecEv E) stk T :=
-  match T return SpecElem E nil T -> tpElem (SpecEv E) stk T with
-  | Tp_M R => fun m => inr (interp_fixtree_nil
-                              (Functor.fmap (liftTpElem (nilListIncl _)) m))
-  | Tp_Pi A B => fun f => inr (fun a => mkTpElem (f a))
-  | Tp_Arr A B =>
-      fun f stk' incl => inr (fun arg => )
-  end.
+End SpecM.
